src/core/DY.Core.Attacker.Knowledge.fst
@@ -159,7 +159,7 @@ let move_requires_4 #a #b #c #d #p #q pf x y z w =
 // (So: any version of a corrupted session is publishable.)
 val corrupted_session_is_publishable:
   {|protocol_invariants|} ->
-  tr:trace -> prin:principal -> sess_id:nat -> content:bytes ->
+  tr:trace -> prin:principal -> sess_id:session_id -> content:bytes ->
   Lemma
   (requires
     is_corrupt tr (principal_state_label prin sess_id) /\
